Verse AST sigT parametrized

src/Verse/Ast.v
@@ -47,20 +47,19 @@ Section VerseCode.
   Variable ts : typeSystem.
 
   Variable v : Variables.U ts.
-  Arguments v [k].
 
   (** Expressions that can occur on the left of an assignment. *)
-  Inductive lexpr : typeOf ts TypeSystem.direct -> Type :=
-  | var   :  forall {ty}, v ty -> lexpr ty
-  | deref :  forall {ty b e}, v (arrayType ts b e ty)-> {i | i < b} -> lexpr ty.
+  Inductive lexpr : some (typeOf ts) -> Type :=
+  | var   :  forall {ty}, v (existT _ direct ty) -> lexpr (existT _ direct ty)
+  | deref :  forall {ty b e}, v (existT _ _ (arrayType ts b e ty)) -> {i | i < b} -> lexpr (existT _ direct ty).
 
   (** The expression type *)
 
-  Inductive expr : typeOf ts TypeSystem.direct -> Type :=
-  | cval     : forall {ty}, constOf ts ty -> expr ty
+  Inductive expr : some (typeOf ts) -> Type :=
+  | cval     : forall {ty}, constOf ts ty -> expr (existT _ direct ty)
   | valueOf  : forall {ty}, lexpr ty -> expr ty
-  | uniOp    : forall {ty}, operator ts ty 1 -> expr ty -> expr ty
-  | binOp    : forall {ty}, operator ts ty 2 -> expr ty -> expr ty -> expr ty
+  | uniOp    : forall {ty}, operator ts ty 1 -> expr (existT _ direct ty) -> expr (existT _ direct ty)
+  | binOp    : forall {ty}, operator ts ty 2 -> expr (existT _ direct ty) -> expr (existT _ direct ty) -> expr (existT _ direct ty)
   .
 
   (** ** Instructions
@@ -91,13 +90,12 @@ Section VerseCode.
 
    *)
 
-  Inductive instruction ty : Type :=
-  | assign      : lexpr ty -> expr ty  -> instruction ty
-  | binopUpdate : lexpr ty -> operator ts ty 2 -> expr ty -> instruction ty
-  | uniopUpdate : lexpr ty -> operator ts ty 1 -> instruction ty
-  | moveTo    : lexpr ty -> v ty  -> instruction ty
-  | clobber   : v ty -> instruction ty.
-
+  Inductive instruction : some (typeOf ts) -> Type :=
+  | assign      kty : lexpr kty -> expr kty  -> instruction kty
+  | binopUpdate ty  : lexpr (existT _ direct ty) -> operator ts ty 2 -> expr (existT _ direct ty) -> instruction (existT _ direct ty)
+  | uniopUpdate ty  : lexpr (existT _ direct ty) -> operator ts ty 1 -> instruction (existT _ direct ty)
+  | moveTo      kty : lexpr kty -> v kty  -> instruction kty
+  | clobber     kty : v kty -> instruction kty.
 
   Definition statement := sigT instruction.
   Definition code := list statement.
@@ -151,7 +149,7 @@ type [ty].
  *)
 Record iterator ts (v : Variables.U ts) (ty : typeOf ts memory)
   := { setup    : code v;
-       process  : v memory ty -> code v;
+       process  : v (existT _ _ ty) -> code v;
        finalise : code v
      }.
 
@@ -163,13 +161,13 @@ Arguments finalise [ts v ty].
 
 Arguments var [ts v ty].
 Arguments deref [ts v ty b e].
-Arguments assign [ts v ty].
+Arguments assign [ts v kty].
 Arguments cval [ts v ty].
 Arguments valueOf [ts v ty].
 Arguments binOp [ts v ty].
 Arguments uniOp [ts v ty].
-Arguments clobber [ts v ty].
-Arguments moveTo [ts v ty].
+Arguments clobber [ts v kty].
+Arguments moveTo [ts v kty].
 Arguments binopUpdate [ts v ty].
 Arguments uniopUpdate [ts v ty].
 
@@ -180,31 +178,34 @@ Require Import Verse.Error.
 Module LExpr.
 
   (** Function for renaming variables *)
-  Definition rename {ts}{u v : Variables.U ts}(rn : Variables.renaming u v) {ty : ts direct} (l : lexpr u ty)
-      := match l with
-         | var x => var (rn direct _ x)
-         | deref a i => deref (rn memory _ a) i
-         end.
+  Definition rename {ts}{u v : Variables.U ts}(rn : Variables.renaming u v) {ty : some (typeOf ts) } (l : lexpr u ty)
+  : lexpr v ty
+    := match l with
+       | var x     => var (rn _ x)
+       | deref a i => deref (rn _ a) i
+       end.
 
   Definition translate src tgt
              (tr : TypeSystem.translator src tgt)
-             (v : Variables.U tgt) (ty : typeOf src direct)
+             (v : Variables.U tgt) (ty : some (typeOf src))
              (le : lexpr (Variables.Universe.coTranslate tr v) ty)
-  : lexpr v (Types.translate tr ty)
-    := match le with
-       | @var _ _ ty x => var (ty := Types.translate tr ty) x
+  : lexpr v (Types.Some.translate tr ty)
+    := match le in lexpr _ ty0 return lexpr _ (Types.Some.translate tr ty0)
+       with
+       | var x => var (ty := Types.translate tr _)
+                      (Variables.translate tr x)
        | @deref _ _ ty b e a i =>
          let compatPf := arrayCompatibility tr b e ty in
          let ap  := Variables.translate tr a in
-         deref (rew compatPf in ap) i
+         deref (rew [fun t => v (existT tgt memory t)] compatPf in ap) i
        end.
 
   Arguments translate [src tgt] tr [v ty].
 
-  Definition result tgt (v : Variables.U tgt) (ty : Types.result tgt direct)
+  Definition result tgt (v : Variables.U tgt) (ty : some (Types.result tgt))
     := match ty with
-       | {- good -} => lexpr v good
-       | error _   => Empty_set + {TranslationError}
+       | existT _ _ {- good -} => lexpr v (existT _ _ good)
+       | existT _ _ (error _)  => Empty_set + {TranslationError}
        end.
 
   Arguments result [tgt].
@@ -212,26 +213,26 @@ Module LExpr.
   Definition extract tgt (v : Variables.U tgt) ty :
     lexpr (Variables.Universe.inject v) ty -> result v ty
     := match ty with
-       | {- good -} => fun l => match l with
-                            | @var _ _ {- good -}  x        => var x
+       | existT _ _ {- good -} => fun l => match l with
+                            | @var _ _ {- good -}  x        => var (ty := good) x
                             | @deref _ _ {- good -} _ _ a i => deref (ty:=good) a i
                             | _ => idProp
                             end
-       | error err
+       | existT _ _ (error err)
          => fun l => error (CouldNotTranslateBecause l err)
        end.
   Arguments extract [tgt v ty].
-(*
+
   Definition compile src tgt
              (cr : TypeSystem.compiler src tgt)
              (v  : Variables.U tgt)
-             (ty : typeOf src direct)
+             (ty : some (typeOf src))
              (le : lexpr (Variables.Universe.coCompile cr v) ty)
-    : result v (Types.compile cr ty)
+    : result v (Types.Some.compile cr ty)
     := extract (translate cr le).
 
   Arguments compile [src tgt] cr [v ty].
- *)
+
 
 
 
@@ -240,7 +241,7 @@ End LExpr.
 Module Expr.
 
   (** Renaming variables in an expression *)
-  Fixpoint rename {ts}{u v : Variables.U ts}(rn : Variables.renaming u v) {ty : ts direct} (e : expr u ty)
+  Fixpoint rename {ts}{u v : Variables.U ts}(rn : Variables.renaming u v) {ty : some ts} (e : expr u ty)
   : expr v ty
     := match e with
          | cval c        => cval c
@@ -252,10 +253,10 @@ Module Expr.
 
   Fixpoint translate {src tgt}
            (tr : TypeSystem.translator src tgt)
-           {v       : Variables.U tgt}
+           {v  : Variables.U tgt}
            {ty}
            (e : expr (Variables.Universe.coTranslate tr v) ty)
-  : expr v (Types.translate tr ty)
+  : expr v (Types.Some.translate tr ty)
     := match e with
          | cval c        => cval (constTrans tr c)
          | valueOf x     => valueOf (LExpr.translate tr x)
@@ -267,10 +268,10 @@ Module Expr.
   Arguments translate [src tgt] tr [v ty].
 
   Definition result tgt
-             (v : Variables.U tgt) (ty : Types.result tgt direct)
+             (v : Variables.U tgt) (ty : some (Types.result tgt))
     := match ty with
-       | {- good -} => expr v good
-       | error _   => Empty_set + {TranslationError}
+       | existT _ _ {- good -} => expr v (existT _ _ good)
+       | existT _ _ (error _)  => Empty_set + {TranslationError}
        end.
   Arguments result [tgt].
 
@@ -282,26 +283,27 @@ Module Expr.
     := match e in expr _ ty0 return result v ty0
        with
        | @cval _ _ {- good -} c        => @cval _ _ good c
-       | @valueOf _ _ {- good -} x     => valueOf (LExpr.extract x)
+       | @valueOf _ _ (existT _ _ {- good -}) x     => valueOf (LExpr.extract x)
        | @binOp _ _ {- good -} o e0 e1 => binOp (ty:=good) o (extract e0) (extract e1)
        | @uniOp _ _ {- good -} o e0    => uniOp (ty:=good) o (extract e0)
        | @cval _ _ (error err) _
-       | @valueOf _ _ (error err) _
+       | @valueOf _ _ (existT _ _ (error err)) _
        | @binOp _ _ (error err) _ _ _
        | @uniOp _ _ (error err) _ _
          => error (CouldNotTranslateBecause e err)
        end.
 
   Arguments extract [tgt v ty].
-  (*
+
+
   Fixpoint compile src tgt
            (cr : TypeSystem.compiler src tgt)
            (v  : Variables.U tgt)
-           (ty : typeOf src direct)
+           (ty : some (typeOf src))
            (e : expr (Variables.Universe.coCompile cr v) ty)
     := extract (translate cr e).
   Arguments compile [src tgt] cr [v ty].
-   *)
+
 End Expr.
 
 Module Instruction.
@@ -310,45 +312,45 @@ Module Instruction.
              (tr : TypeSystem.translator src tgt)
              (v : Variables.U tgt)
              ty (i : instruction (Variables.Universe.coTranslate tr v) ty)
-  : instruction v (Types.translate tr ty) :=
+  : instruction v (Types.Some.translate tr ty) :=
     match i with
     | assign x e => assign (LExpr.translate tr x) (Expr.translate tr e)
     | binopUpdate x o e0 => binopUpdate (LExpr.translate tr x) (opTrans tr o) (Expr.translate tr e0)
     | uniopUpdate x o    => uniopUpdate (LExpr.translate tr x) (opTrans tr o)
-    | moveTo x y  => (fun yp : v direct (Types.translate tr ty) => moveTo (LExpr.translate tr x) yp) y
-    | clobber x   => (fun xp : v direct (Types.translate tr ty) => clobber xp) x
+    | @moveTo _ _ kty x y  => (fun yp : v (Types.Some.translate tr kty) => moveTo (LExpr.translate tr x) yp) y
+    | @clobber _ _ kty x   => (fun xp : v (Types.Some.translate tr kty) => clobber xp) x
     end.
 
   Arguments translate [src tgt] tr [v ty].
   Definition result tgt
              (v  : Variables.U tgt)
-             (ty : Types.result tgt direct)
+             (ty : some (Types.result tgt))
     := match ty with
-       | {- tyc -} => instruction v tyc
-       | error _   => Empty_set + {TranslationError}
+       | existT _ _ {- tyc -} => instruction v (existT _ _ tyc)
+       | existT _ _ (error _) => Empty_set + {TranslationError}
        end.
 
   Arguments result [tgt].
 
   Definition extract tgt
              (v : Variables.U tgt)
-             (ty : Types.result tgt direct)
+             (ty : some (Types.result tgt))
     : instruction (Variables.Universe.inject v) ty -> result v ty
     := match ty with
-       | error err =>  fun i => error (CouldNotTranslateBecause i err)
-       | {- good -} =>
-           let lext := LExpr.extract (ty:={- good -}) in
-           let ext  := Expr.extract (ty:={- good -}) in
-           fun i =>
-               match i with
-               | assign x e => assign (lext x) (ext e)
-               | binopUpdate x o e0 => binopUpdate (lext x) o (ext e0)
-               | uniopUpdate x o  => uniopUpdate (lext x) o
-               | moveTo x y  => moveTo (lext x) y
-               | clobber x   => clobber x
+       | existT _ _ (error err) =>  fun i => error (CouldNotTranslateBecause i err)
+       | existT _ _ {- good -} as ty0 =>
+           fun i : instruction _ ty0 =>
+             (* TODO : Surely the following match can be written better *)
+             match i in instruction _ ty0
+             with
+               | @assign _ _ (existT _ _ {-g-}) x e => assign (LExpr.extract x) (Expr.extract e)
+               | @binopUpdate _ _ {-g-} x o e0 => binopUpdate (LExpr.extract x) o (Expr.extract e0)
+               | @uniopUpdate _ _ {-g-} x o  => uniopUpdate (LExpr.extract x) o
+               | @moveTo _ _ (existT _ _ {-g-}) x y  => moveTo (LExpr.extract x) y
+               | @clobber _ _ (existT _ _ {-g-}) x   => clobber (kty := existT _ _ g) x
+               | _ => idProp
                end
-
-         end.
+           end.
 
   Arguments extract [tgt v ty].
 
@@ -387,16 +389,16 @@ Module Statement.
              (v : Variables.U tgt)
              (s : statement (Variables.Universe.coCompile cr v))
              : result v
-    := match Types.translate cr (projT1 s) as ty0
-             return Types.translate cr (projT1 s) = ty0
+    := match Types.Some.translate cr (projT1 s) as ty0
+             return Types.Some.translate cr (projT1 s) = ty0
                     -> result v
        with
-       | {- good -}
-         => fun tyeq => {- existT _ good
+       | existT _ _ {- good -}
+         => fun tyeq => {- existT _ (existT _ _ good)
                                   (rew [Instruction.result _] tyeq
                                     in
                                       (Instruction.compile _ (projT2 s))) -}
-       | error _
+       | existT _ _ (error _)
          => fun _ => error (CouldNotTranslate s)
        end eq_refl.
 
@@ -480,13 +482,12 @@ Module Iterator.
              (itr : iterator (Variables.Universe.coCompile cr v) memty)
              (good : typeOf tgt memory)
              (pf : Types.compile cr memty = {- good -})
-             (x  : v memory good)
+             (x  : v (existT _ _ good))
     : compiled tgt v + {TranslationError}
-    := (do stup <- Code.compile cr (setup itr) ;;
-        do fnls <- Code.compile cr (finalise itr) ;;
-        do prcs <- Code.compile cr (process itr (rew <- pf in Variables.inject x)) ;;
-           pure {| preamble := stup;  loopBody := prcs; finalisation := fnls |}
-       ).
+    := do stup <- Code.compile cr (setup itr) ;;
+       do fnls <- Code.compile cr (finalise itr) ;;
+       do prcs <- Code.compile cr (process itr (rew <- f_equal _ pf in Variables.inject x)) ;;
+          pure {| preamble := stup;  loopBody := prcs; finalisation := fnls |}.
 
   Arguments compile [src tgt] cr [v memty] itr [good].
 
